Have.v
@@ -2,6 +2,7 @@ Require Import Omega.
 
 Class Have (P : Prop) := have : P.
 
-Hint Extern 4 (Have ?P) => unfold Have in * ; omega : typeclass_instances.
-
 Ltac unhave := unfold Have in *.
+
+Hint Extern 4 (Have ?P) => unhave ; omega : typeclass_instances.
+
