SPARC.v
@@ -1,18 +1,42 @@
-Require Import CSDL.Binary CSDL.Representable CSDL.csdl.
+Require Import CSDL.Binary CSDL.BinaryBe CSDL.Representable CSDL.Range CSDL.csdl.
 
-Program Definition i : space := 
+Program Definition i : space_descr := 
  {| space_name := "control/status registers";
     space_address := 3;
     space_cell_size := 32;
     space_n := Some (existT _ 6 (representation 3 6))
  |}.
 
+  Next Obligation. unhave; omega. Defined.
+
 About exp.
 About eval_exp.
-Definition sharp (s : space) {n} (e : exp n) : loc n := 
-  
+About mem_cell_fetch.
+Definition sharp (s : space_descr) (e : exp (s.(space_address))) : interpM (loc s) := 
+  eval_exp e.
+    
+Delimit Scope exp_scope with exp.
 
-Definition loc1 := $i[0].
+Notation " # s [ e ] " := (sharp s e%exp) (s ident).
+
+Notation "0" := zero : exp_scope.
+Notation "1" := one : exp_scope.
+
+Coercion CONST : const >-> exp.
+
+Definition bits_const {n} (b : bits n) : exp n :=
+  CONST b.
+
+Coercion bits_const : bits >-> exp.
+
+About representation_range.
+
+Definition loc1 := #i[0].
+Definition loc2 := #i[1].
+
+Definition loc12 := #i[representation_range (range_of_bounds 0 1) _].
+
+Print loc1.
 
 
   
