Validator.v
@@ -1,0 +1,348 @@
+Require Import Equations.
+
+Equations(nocomp) nth_prf {A} (n : nat) (l : list A) (p : n < length l) : A :=
+nth_prf A n nil pf :=! pf;
+nth_prf A O (cons a l) pf := a ;
+nth_prf A (S n) (cons a l) pf := nth_prf n l _.
+
+  Next Obligation. inversion pf. Defined.
+  Next Obligation. auto with arith. Defined.
+  Next Obligation. find_empty. Defined.
+
+Require Import Asm.X86.X86.
+Require Import Asm.Bitvector.Bitvector.
+Require Import String.
+Require Import Bvector.
+Require Import CSDL.Vector.
+Require Import CSDL.Binary.
+Require Import CSDL.Representable.
+Require Import CSDL.BinaryBe.
+
+Definition regset := Int32Map.t bool.
+
+Definition instr_is_disallowed (i : instr) :=
+  match i with
+    (* Disallow [ret] and indirect calls through memory. *)
+    | Ret => true
+    | Call op | Jmp op =>
+      match op with
+        | Address _ => true
+        | _ => false
+      end
+    | _ => false
+  end.
+
+Require Import CSDL.Hexadecimal.
+Require Import CSDL.Show.
+
+Definition cs_mask : bits 32 :=
+  fst (binary_minus_be full (representation 32 31)).
+
+Eval vm_compute in (eq_refl : print cs_mask = "0xffffffe0")%string.
+
+Definition nacl_jmp_instr : (instr * instr) :=
+  (Arith And (Reg EAX) (Imm _ cs_mask), Jmp (Reg EAX)).
+
+Require Import EquivDec.
+
+Instance: EqDec int32 eq.
+Proof. apply const_eq. Defined.
+
+Ltac dec_eq_one := 
+  match goal with 
+    | H : ?x =/= ?x |- _ => elimtype False; apply H; reflexivity
+    | H : ?x === ?y |- _ => red in H; subst
+    | |- { ?x === ?x } + { _ } => left; reflexivity
+    | |- { _ } + { ?x =/= ?x } => left; f_equal
+    | |- { ?x === ?y } + { _ } => right; let H := fresh in intro H; red in H; 
+      (injection H || discriminate); intros; subst
+  end.
+
+Ltac dec_eq := try solve [ repeat dec_eq_one ];
+  repeat match goal with H : _ === _ |- _ => red in H; subst end.
+
+Instance option_eq_dec {A} `(EqDec A eq) : EqDec (option A) eq.
+Proof.
+  intros x y. destruct x; destruct y; dec_eq.
+  destruct (equiv_dec a a0); dec_eq. 
+Qed.
+
+Instance reg32_eq_dec : EqDec reg32 eq.
+  intros x y. apply reg32_eq_dec. 
+Qed.
+
+Instance reg8_eq_dec : EqDec reg8 eq.
+  intros x y. change ({x = y} + {x <> y}).
+  decide equality x y. 
+Qed.
+
+Instance scale_eq_dec : EqDec scale eq.
+  intros x y. change ({x = y} + {x <> y}). 
+  decide equality x y.
+Qed.
+
+Instance: EqDec address eq. 
+  red; intros. destruct x; destruct y; dec_eq.
+  destruct (equiv_dec addrDisp addrDisp0); dec_eq.
+  destruct (equiv_dec addrBase addrBase0); dec_eq.
+  destruct (equiv_dec addrIndex addrIndex0); dec_eq.
+Qed.
+
+Instance genop_eq_dec : EqDec genop32 eq.
+  intros x y. change ({x = y} + {x <> y}).
+  decide equality x y. 
+  apply int32_eq_dec. apply reg32_eq_dec. 
+  apply equiv_dec.
+Qed.
+
+Instance genop8_eq_dec : EqDec genop8 eq.
+  intros x y. change ({x = y} + {x <> y}).
+  decide equality x y. 
+  apply int32_eq_dec. apply reg8_eq_dec. 
+  apply equiv_dec.
+Qed.
+
+Instance arith_op_eq_dec : EqDec arith_op eq.
+  intros x y. change ({x = y} + {x <> y}).
+  decide equality x y. 
+Qed.
+
+Instance condition_eq_dec : EqDec condition eq.
+  intros x y. change ({x = y} + {x <> y}).
+  decide equality x y. 
+Defined.
+
+Instance cc_eq_dec : EqDec cc eq.
+  intros x y. change ({x = y} + {x <> y}).
+  decide equality x y. 
+  apply condition_eq_dec.
+  apply equiv_dec.
+Qed.
+
+Instance shift_op_eq_dec : EqDec shift_op eq.
+  intros x y. change ({x = y} + {x <> y}).
+  decide equality x y. 
+Qed.
+
+Instance instr_eq_dec : EqDec instr eq.
+  intros x y. 
+  destruct x; destruct y; dec_eq.
+  Ltac add_eq :=
+    match goal with
+      | [ x : ?T, y : ?T |- _ ] =>
+        match goal with 
+          | H : x === y |- _ => red in H; subst
+          | _ => destruct (equiv_dec x y)
+        end
+    end. 
+  destruct (equiv_dec a a0); dec_eq.
+  destruct (equiv_dec g g1); dec_eq.
+  destruct (equiv_dec g0 g2); dec_eq.
+
+  destruct (equiv_dec a a0); dec_eq.
+  destruct (equiv_dec g g1); dec_eq.
+  destruct (equiv_dec g0 g2); dec_eq.
+
+  destruct (equiv_dec g g0); dec_eq.
+
+  destruct (equiv_dec g g1); dec_eq.
+  destruct (equiv_dec g0 g2); dec_eq.
+
+  destruct (equiv_dec g g0); dec_eq.
+
+  destruct (equiv_dec i i0); dec_eq.
+  destruct (equiv_dec c c0); dec_eq.
+
+  destruct (equiv_dec g g0); dec_eq.
+
+  destruct (equiv_dec r r0); dec_eq.
+  destruct (equiv_dec a a0); dec_eq.
+
+  destruct (equiv_dec g g1); dec_eq.
+  destruct (equiv_dec g0 g2); dec_eq.
+
+  destruct (equiv_dec g g1); dec_eq.
+  destruct (equiv_dec g0 g2); dec_eq.
+
+  destruct (equiv_dec g g0); dec_eq.
+
+  destruct (equiv_dec g g0); dec_eq.
+
+  destruct (equiv_dec s s0); dec_eq.
+  destruct (equiv_dec g g1); dec_eq.
+  destruct (equiv_dec g0 g2); dec_eq.
+Defined.
+
+Definition is_nacl_jmp_idiom i j :=
+  let '(a, b) := nacl_jmp_instr in
+    equiv_decb a i && equiv_decb b j.
+
+Definition block_size := 32. (* bytes *)
+Definition block_size_bin : bits 32 := 
+  representation (e:=BigEndian) 32 32.
+Definition block_size_mask : bits 32 :=
+  binary_shiftl_n_full full 5.
+
+Definition block (ip : int32) : int32 :=
+  BVand 32 ip (vector_append (full (n:=30)) (zero (n:=2))).
+
+Parameter decode_instr : int32 -> instr * int32.
+Parameter instr_length : int32 -> int32.
+
+Definition instr_overlaps_block_size (ip : int32) : bool :=
+  let (instrend, of) := binary_plus_be ip (instr_length ip) in
+    of || negb (binary_eq zero (BVand 32 block_size_mask instrend)).
+
+Definition instr_is_indirect_jmp_or_call (i : instr) :=
+  match i with
+    | Jmp (Imm _)
+    | Call (Imm _) => false
+    | Jmp _ | Call _ => true
+    | _ => false
+  end.
+
+Definition instr_is_direct_jmp_or_call (i : instr) : option int32 :=
+  match i with
+    | Jmp (Imm ip) => Some ip
+    | Call (Imm ip) => Some ip
+    | _ => None
+  end.
+
+Inductive valid_error : Set :=
+| Disallowed_instruction
+| Block_alignment_failure
+| Bad_indirect_control
+| Call_to_invalid_address.
+Print sum.
+
+Definition start_addresses := list int32.
+
+Definition two {n} : bits (Datatypes.S (Datatypes.S n)) :=
+  zx_be (Vcons true (Vcons false Vnil)).
+
+(* Equations(nocomp) build_startaddrs (ip : int32) (jtargets : regset) *)
+(*   (sa : start_addresses) *)
+(*   (icount : nat) (instrs : list instr) (p : bvec_to_nat ip < length instrs) *)
+(*   { measure (length instrs - icount) } : (regset * start_addresses) + valid_error := *)
+(*   if eq_nat_dec (Datatypes.S (bvec_to_nat ip)) (length instrs) then inl (jtargets, sa) *)
+(*   else *)
+(*     let instr := nth_prf (bvec_to_nat ip) instrs p in *)
+(*       if instr_is_disallowed instr  *)
+(*       then inr Disallowed_instruction *)
+(*       else *)
+(*         let sa := ip :: sa in *)
+(*         let jtargets := Int32Map.set ip true jtargets in *)
+(*           if instr_overlaps_block_size ip *)
+(*           then inr Block_alignment_failure *)
+(*           else if instr_is_indirect_jmp_or_call instr  *)
+(*             then if ltb icount 2  *)
+(*               then inr Bad_indirect_control *)
+(*               else if negb (binary_eq (block ip) (block (bdec (bdec ip))))  *)
+(*                 then inr Bad_indirect_control *)
+(*                 else if negb (is_nacl_jmp_idiom instr (nth_prf (bvec_to_nat (bdec ip)) instrs _))  *)
+(*                 then inr Bad_indirect_control *)
+(*                 else build_startaddrs (binc ip) jtargets sa (Datatypes.S icount) instrs _ *)
+(*             else build_startaddrs (binc ip) jtargets sa (Datatypes.S icount) instrs _. *)
+
+Section Validator.
+  Variable text_limit : int32.
+  
+  Program Fixpoint build_startaddrs (ip : int32) (jtargets : regset) (sa : start_addresses) 
+    (prev : list instr) (instrs : list instr) { struct instrs } 
+    : (regset * start_addresses) + valid_error :=
+    match instrs with
+      | nil => inl (jtargets, sa)
+      | cons instr instrs =>
+        if instr_is_disallowed instr 
+        then inr Disallowed_instruction
+        else
+          let sa := ip :: sa in
+          let jtargets := Int32Map.set ip true jtargets in
+            if instr_overlaps_block_size ip
+            then inr Block_alignment_failure
+            else if instr_is_indirect_jmp_or_call instr 
+              then if dec (ltb (List.length prev) 2)
+                then inr Bad_indirect_control
+                else if negb (binary_eq (block ip) (block (bdec (bdec ip)))) 
+                  then inr Bad_indirect_control
+                  else if negb (is_nacl_jmp_idiom instr (nth_prf (bvec_to_nat (bdec ip)) instrs _)) 
+                  then inr Bad_indirect_control
+                  else build_startaddrs (binc ip) jtargets sa (instr :: prev) instrs
+              else build_startaddrs (binc ip) jtargets sa (instr :: prev) instrs
+    end.
+
+  Next Obligation. admit. Defined.
+
+
+(* Program Fixpoint build_startaddrs (ip : int32) (jtargets : regset) *)
+(*   (sa : start_addresses) *)
+(*   (icount : nat) (instrs : list instr) (p : bvec_to_nat ip < length instrs) *)
+(*   { measure (length instrs - icount) } : (regset * start_addresses) + valid_error := *)
+(*   if eq_nat_dec (Datatypes.S (bvec_to_nat ip)) (length instrs) then inl (jtargets, sa) *)
+(*   else *)
+(*     let instr := nth_prf (bvec_to_nat ip) instrs p in *)
+(*       if instr_is_disallowed instr  *)
+(*       then inr Disallowed_instruction *)
+(*       else *)
+(*         let sa := ip :: sa in *)
+(*         let jtargets := Int32Map.set ip true jtargets in *)
+(*           if instr_overlaps_block_size ip *)
+(*           then inr Block_alignment_failure *)
+(*           else if instr_is_indirect_jmp_or_call instr  *)
+(*             then if ltb icount 2  *)
+(*               then inr Bad_indirect_control *)
+(*               else if negb (binary_eq (block ip) (block (bdec (bdec ip))))  *)
+(*                 then inr Bad_indirect_control *)
+(*                 else if negb (is_nacl_jmp_idiom instr (nth_prf (bvec_to_nat (bdec ip)) instrs _))  *)
+(*                 then inr Bad_indirect_control *)
+(*                 else build_startaddrs (binc ip) jtargets sa (Datatypes.S icount) instrs _ *)
+(*             else build_startaddrs (binc ip) jtargets sa (Datatypes.S icount) instrs _. *)
+
+(*   Next Obligation. *)
+(* Admitted. *)
+
+(*   Next Obligation. *)
+(*     admit. *)
+(*   Defined. *)
+
+(*   Next Obligation.  *)
+(*     admit. *)
+(*   Defined. *)
+
+(*   Next Obligation.  *)
+(*     admit. *)
+(*   Defined. *)
+
+(*   Next Obligation.  *)
+(*     admit. *)
+(*   Defined. *)
+
+    Fixpoint direct_transfers (l : list instr) (jtargets : regset) (sa : start_addresses) : unit + valid_error :=
+      match sa with
+        | nil => inl tt
+        | cons ip sas =>
+          let instr := List.nth (bvec_to_nat ip) l Ret in
+            match instr_is_direct_jmp_or_call instr with
+              | Some ip' => 
+                if negb (binary_be_lt ip' text_limit) 
+                  || negb (Int32Map.get ip' jtargets)
+                then inr Call_to_invalid_address
+                else direct_transfers l jtargets sas
+              | None => direct_transfers l jtargets sas
+            end
+      end.
+
+    Definition validator (s : list instr) : unit + valid_error :=
+      let jump_targets := Reg32Map.init false in
+      let ip : int32 := nat_to_bvec 32 0 in
+        match build_startaddrs zero jump_targets [] [] s with
+          | inl (targets, sa) =>
+            direct_transfers s targets sa
+          | inr r => inr r
+        end.
+
+End Validator.
+
+
+
+    
